\documentclass[]{article}
\usepackage{amsmath}
\usepackage{amsbsy}
\usepackage{breqn}
\usepackage[margin=0.5in]{geometry}

\newcommand{\mbrack}[1]{\left\lbrack #1 \right\rbrack}
\newcommand{\mbrace}[1]{\left\lbrace #1 \right\rbrace}
\newcommand{\mparen}[1]{\left(#1\right)}

%opening
\title{Derivation of SLDA Variational Inference}
\author{}

\begin{document}

\maketitle

\section*{Derivation of Variational Spatial LDA}

Terminology
\begin{itemize}
	\item Bold $\boldsymbol{var}$ for observed variables
\end{itemize}

Variational Distribution
\begin{eqnarray}
q(\phi,\pi,d,z | \lambda,\gamma,\rho,\xi) &=& \prod\limits_{k=1}^{K}q(\phi_k|\lambda) \: \prod\limits_{m=1}^{M}q(\pi_m|\gamma) \: \prod\limits_{n=1}^{N}q(d_n | \rho) q(z_n | \xi)
\end{eqnarray}
where 
\begin{itemize}
	\item[$\phi_k \in R^V$] distribution over word of topic $k$
	\item[$\pi_m \in R^K$] distribution over topics of document $m$
	\item[$d_n \in R^M$] indicator vector where if $d_{nm} = 1$ means word $n$ belongs to document $m$
	\item[$z_n \in R^K$] indicator vector where if $z_{nk} = 1$ means word $n$ is assigned to topic $k$
\end{itemize}

Lower bound of log likelihood:
\begin{eqnarray}
p(\boldsymbol{w}, \boldsymbol{c} | \alpha,\beta,\eta,\sigma) 
&=& \log \int\limits_{\phi} \int\limits_{\pi} \sum\limits_{d} \sum\limits_{z} p(\phi,\pi,d,z,\boldsymbol{w},\boldsymbol{c} | \alpha,\beta,\eta,\sigma) \\
&=&  \log \int\limits_{\phi} \int\limits_{\pi} \sum\limits_{d} \sum\limits_{z} q(\phi,\pi,d,z | \lambda,\gamma,\rho,\xi) \frac{p(\phi,\pi,d,z,\boldsymbol{c},\boldsymbol{w} | \alpha,\beta,\eta,\sigma)}{q(\phi,\pi,d,z | \lambda,\gamma,\rho,\xi)} \; \mathrm{d}\phi \: \mathrm{d}\pi \: \mathrm{d}d \: \mathrm{d}z\\
&=& \log E_q \frac{p(\phi,\pi,d,z,\boldsymbol{c},\boldsymbol{w} | \alpha,\beta,\eta,\sigma)}{q(\phi,\pi,d,z | \lambda,\gamma,\rho,\xi)} \\
&\ge& E_q \log p(\phi,\pi,d,z,\boldsymbol{c},\boldsymbol{w} | \alpha,\beta,\eta,\sigma) - E_q \log q(\phi,\pi,d,z | \lambda,\gamma,\rho,\xi) = L
\end{eqnarray}
where $E_q \equiv E_{q(\phi,\pi,d,z | \lambda,\gamma,\rho,\xi)}$

Instead of maximizing $p$, we estimate it by maximizing the lower bound $L$

\subsection*{First Term in $L$}

\begin{eqnarray}
E_q [\log p(\phi,\pi,d,z,\boldsymbol{c},\boldsymbol{w} | \alpha,\beta,\eta,\sigma)] &=& E_q [\log p(\phi|\beta) \: p(\pi|\alpha) \: p(d | \eta) \: p(\boldsymbol{c} | c^{\mathrm{d}}_d, \sigma) \: p(z | \pi_d) \: p(\boldsymbol{w} | \phi_d) \\
&=& E_q [\log p(\phi|\beta)] + E_q [\log p(\pi|\alpha)] + E_q [\log p(d | \eta)] \\
&+& E_q [\log p(\boldsymbol{c} | c^{\mathrm{d}}_d, \sigma)] + E_q[\log p(z | \pi_d)] + E_q [\log p(\boldsymbol{w} | \phi_z)] \\
\end{eqnarray}

For each sub-terms:

\begin{eqnarray}
E_q [\log p(\phi|\beta)] 
&=& E_q \lbrack \log \prod\limits_{k=1}^{K} p(\phi_k | \beta) \rbrack \\
&=& \sum\limits_{k=1}^{K} E_q \left\lbrack \log \Gamma \left( \sum\limits_{v=1}^{V} \beta_{v} \right) - \sum\limits_{v=1}^{V} \log \Gamma(\beta_{v}) + \sum\limits_{v=1}^{V} (\beta_{v}-1) \log(\phi_{kv}) \right\rbrack \\
&=& \sum\limits_{k=1}^{K} \left\lbrack \log \Gamma(\sum\limits_{v=1}^{V} \beta_{v}) - \sum\limits_{v=1}^{V} \log \Gamma(\beta_{v}) + \sum\limits_{v=1}^{V} (\beta_{v}-1) (\Psi(\lambda_{kv}) - \Psi(\sum\limits_{v^'=1}^{V} \lambda_{kv^'})) \right\rbrack
\end{eqnarray}

\begin{eqnarray}
E_q [\log p(\pi|\alpha)] 
&=& E_q [\log \prod\limits_{m=1}^{M} p(\pi_m |  \alpha)] \\
&=& \sum\limits_{m=1}^{M} E_q \log(p(\pi_m|\alpha)) \\
&=& \sum\limits_{m=1}^{M} E_q \left\lbrack \log(\Gamma\mparen{\sum\limits_{k=1}^{K} \alpha_{k}}) - \sum\limits_{k=1}^{K} \log(\Gamma(\alpha_{k})) + \sum\limits_{k=1}^{K} (\alpha_{k}-1) \log(\pi_{mk}) \right\rbrack \\
&=& \sum\limits_{m=1}^{M} \left\lbrack \log(\Gamma(\mparen{\sum\limits_{k=1}^{K} \alpha_{k}}) - \sum\limits_{k=1}^{K} \log(\Gamma(\alpha_{k})) + \sum\limits_{k=1}^{K} (\alpha_{k}-1) (\Psi(\gamma_{mk}) - \Psi(\sum\limits_{k'=1}^{K} \gamma_{mk'})) \right\rbrack\\
\end{eqnarray}

The following derivations skip some steps for the purpose of shorter writings.

\begin{eqnarray}
E_q [\log p(d | \eta)] 
&=& \sum\limits_{n=1}^{N} E_q \log(p(d_n | \eta)) \\
&=& \sum\limits_{n=1}^{N} E_q \left\lbrack \sum\limits_{m=1}^{M} d_{mn} \log(\eta) \right\rbrack\\
&=& \sum\limits_{n=1}^{N} \sum\limits_{m=1}^{M} \rho_{mn} \log(\eta) \\
\end{eqnarray}

\textit{$c_{d_n}^{\mathrm{d}}$: location of document d (in its image)}.

\begin{eqnarray}
E_q [\log p(\boldsymbol{c} | c^{\mathrm{d}}_d, \sigma)] 
&=& \sum\limits_{n=1}^{N} E_q \log p(c_n | c_{d_n}^{\mathrm{d}}) \\
&=& \sum\limits_{n=1}^{N} E_q \left\lbrack \sum\limits_{m=1}^{M}  d_{mn} \log p(c_n | c_{d_{mn}}^{\mathrm{d}}) \right\rbrack \\
&=& \sum\limits_{n=1}^{N} \sum\limits_{m=1}^{M} E_q [d_{mn} \log p(c_n | c_{d_{mn}}^{\mathrm{d}})]  \\
&=& \sum\limits_{n=1}^{N} \sum\limits_{m=1}^{M} \rho_{mn} (\log \delta_{g_{d_{mn}}^{\mathrm{d}}} - \frac{(x_{d_{mn}}^{\mathrm{d}} - x_n)^2 + (y_{d_{mn}}^{\mathrm{d}} - y_n)^2}{\sigma^2})\\
\end{eqnarray}

\begin{eqnarray}
E_q[\log p(z | \pi_d)]
&=& \sum\limits_{n=1}^{N} E_q \left\lbrack \sum\limits_{m=1}^{M} \sum\limits_{k=1}^{K} d_{mn} z_{kn} \log(\pi_{mk}) \right\rbrack \\
&=& \sum\limits_{n=1}^{N} \sum\limits_{m=1}^{M} \sum\limits_{k=1}^{K} E_q[d_{mn} z_{kn} \log(\pi_{mk})] \\
&=& \sum\limits_{n=1}^{N} \sum\limits_{m=1}^{M} \sum\limits_{k=1}^{K} \rho_{mn} \xi_{kn} (\Psi(\gamma_{mk}) - \Psi(\sum\limits_{m'=1}^{M} \gamma_{m'k}))
\end{eqnarray}

\begin{eqnarray}
E_q [\log p(\boldsymbol{w} | \phi_z)]
&=& \sum\limits_{n}^{N} E_q \left\lbrack \sum\limits_{m}^{M} \sum\limits_{k}^{K} \sum\limits_{v}^{V} d_{mn} z_{kn} w^v_n log(\phi_{kv}) \right\rbrack \\
&=& \sum\limits_{n}^{N} \sum\limits_{m}^{M} \sum\limits_{k}^{K} \sum\limits_{v}^{V} E_q[d_{mn} z_{kn} w^v_n log(\phi_{kv})] \\
&=& \sum\limits_{n}^{N} \sum\limits_{m}^{M} \sum\limits_{k}^{K} \sum\limits_{v}^{V} \rho_{mn} \xi_{kn} w_n^v (\Psi(\lambda_{k\boldsymbol{v}}) - \Psi(\sum\limits_{k'}^{K} \lambda_{k'\boldsymbol{v}})) \\
\end{eqnarray}

\subsection*{The second term in $L$}

This uses the log of the joint distribution under variational parameters in (1)

\begin{eqnarray}
E_q \log q(\phi | \lambda) 
&=& \sum\limits_{k}^{K} E_q \log q(\phi_k | \lambda) \\
&=& \sum\limits_{k}^{K} \mbrack{\log \Gamma(\sum\limits_{v}^{V} \lambda_{kv}) - \sum\limits_{v}^{V} \log(\Gamma(\lambda_{kv})) + \sum\limits_{v}^{V}(\lambda_{kv}-1) E_q[\log(\phi_{kv})]} \\
&=& \sum\limits_{k}^{K} \left\lbrack \log \Gamma \mparen{\sum\limits_{v}^{V} \lambda_{kv}} - \sum\limits_{v}^{V} \log(\Gamma(\lambda_{kv})) + \sum\limits_{v}^{V}(\lambda_{kv}-1)(\Psi(\lambda_{kv}) - \Psi(\sum\limits_{v'}^{V} \lambda_{kv'}) \right\rbrack \\
\end{eqnarray}

\begin{eqnarray}
E_q \log q(\pi | \gamma) 
&=& \sum\limits_{m}^{M} E_q \log q(\pi_m | \gamma) \\
&=& \sum\limits_{m}^{M} \mbrack{ \log \Gamma \mparen{ \sum\limits_{k}^{K} \gamma_{km}} - \sum\limits_{k}^{K} \log \Gamma(\gamma_{km}) + \sum\limits_{k}^{K}(\gamma_{km}-1)E_q[\log(\pi_{km})] } \\
&=& \sum\limits_{m}^{M} \mbrack{ \log \Gamma\mparen{ \sum\limits_{k}^{K} \gamma_{km}} - \sum\limits_{k}^{K} \log \Gamma(\gamma_{km}) + \sum\limits_{k}^{K}(\gamma_{km}-1)(\Psi(\gamma_{km}) - \Psi(\sum\limits_{k'}^{K} \gamma_{k'm})) }\\
\end{eqnarray}

\begin{eqnarray}
E_q \log q(d | \rho) 
&=& \sum\limits_{n}^{N} E_q [\log p(d_n | \rho)] \\
&=& \sum\limits_{n}^{N} \sum\limits_{m}^{M} E_q [d_{mn} \log(\rho_{mn})] \\
&=& \sum\limits_{n}^{N} \sum\limits_{m}^{M} \rho_{mn} \log(\rho_{mn}) \\
\end{eqnarray}

\begin{eqnarray}
E_q \log q(z | \xi) 
&=& \sum\limits_{n}^{N} E_q \log q(z_n | \xi) \\
&=& \sum\limits_{n}^{N} \sum\limits_{k}^{K} E_q [z_{kn} \log(\xi_{kn})] \\
&=& \sum\limits_{n}^{N} \sum\limits_{k}^{K} \xi_{kn} \log(\xi_{kn})\\
\end{eqnarray}

\newpage

\subsection*{Putting it all together}

\begin{eqnarray}
L 
&=& \sum\limits_{k=1}^{K} \left\lbrack \log \Gamma(\sum\limits_{v=1}^{V} \beta_{v}) - \sum\limits_{v=1}^{V} \log \Gamma(\beta_{v}) + \sum\limits_{v=1}^{V} (\beta_{v}-1) (\Psi(\lambda_{kv}) - \Psi(\sum\limits_{v^'=1}^{V} \lambda_{kv^'})) \right\rbrack \\
&+& \sum\limits_{m=1}^{M} \left\lbrack \log(\Gamma(\sum\limits_{k=1}^{K} \alpha_{k})) - \sum\limits_{k=1}^{K} \log(\Gamma(\alpha_{k})) + \sum\limits_{k=1}^{K} (\alpha_{k}-1) (\Psi(\gamma_{mk}) - \Psi(\sum\limits_{k'=1}^{K} \gamma_{mk'})) \right\rbrack \\
&+& \sum\limits_{n=1}^{N} \sum\limits_{m=1}^{M} \rho_{mn} \log(\eta) \\
&+& \sum\limits_{n=1}^{N} \sum\limits_{m=1}^{M} \rho_{mn} (\log \delta_{g_{d_{mn}}^{\mathrm{d}}} - \frac{(x_{d_{mn}}^{\mathrm{d}} - x_n)^2 + (y_{d_{mn}}^{\mathrm{d}} - y_n)^2}{\sigma^2}) \\
&+& \sum\limits_{n=1}^{N} \sum\limits_{m=1}^{M} \sum\limits_{k=1}^{K} \rho_{mn} \xi_{kn} (\Psi(\gamma_{mk}) - \Psi(\sum\limits_{m'=1}^{M} \gamma_{m'k})) \\
&+& \sum\limits_{n}^{N} \sum\limits_{m}^{M} \sum\limits_{k}^{K} \sum\limits_{v}^{V} \rho_{mn} \xi_{kn} w_n^v (\Psi(\lambda_{k\boldsymbol{v}}) - \Psi(\sum\limits_{k'}^{K} \lambda_{k'\boldsymbol{v}})) \\
&-& \sum\limits_{k}^{K} \left\lbrack \log \Gamma \mparen{\sum\limits_{v}^{V} \lambda_{kv}} - \sum\limits_{v}^{V} \log(\Gamma(\lambda_{kv})) + \sum\limits_{v}^{V}(\lambda_{kv}-1)(\Psi(\lambda_{kv}) - \Psi(\sum\limits_{v'}^{V} \lambda_{kv'}) \right\rbrack \\
&-& \sum\limits_{m}^{M} \mbrack{ \log \Gamma\mparen{ \sum\limits_{k}^{K} \gamma_{km}} - \sum\limits_{k}^{K} \log \Gamma(\gamma_{km}) + \sum\limits_{k}^{K}(\gamma_{km}-1)(\Psi(\gamma_{km}) - \Psi(\sum\limits_{k'}^{K} \gamma_{k'm})) }\\
&-& \sum\limits_{n}^{N} \sum\limits_{m}^{M} \rho_{mn} \log(\rho_{mn}) \\
&-& \sum\limits_{n}^{N} \sum\limits_{k}^{K} \xi_{kn} \log(\xi_{kn})\\
\end{eqnarray}

Maximize with respect to each term:

\begin{eqnarray}
L_{\rho_{mn}} 
&=&\sum\limits_{n=1}^{N} \sum\limits_{m=1}^{M} \rho_{mn} \log(\eta) \\
&+& \sum\limits_{n=1}^{N} \sum\limits_{m=1}^{M} \rho_{mn} (\log \delta_{g_{d_{mn}}^{\mathrm{d}}} - \frac{(x_{d_{mn}}^{\mathrm{d}} - x_n)^2 + (y_{d_{mn}}^{\mathrm{d}} - y_n)^2}{\sigma^2})\\
&+& \sum\limits_{n=1}^{N} \sum\limits_{m=1}^{M} \sum\limits_{k=1}^{K} \rho_{mn} \xi_{kn} (\Psi(\gamma_{mk}) - \Psi(\sum\limits_{m'=1}^{M} \gamma_{m'k}) \\
&+& \sum\limits_{n}^{N} \sum\limits_{m}^{M} \sum\limits_{k}^{K} \sum\limits_{v}^{V} \rho_{mn} \xi_{kn} w_n^v (\Psi(\lambda_{k\boldsymbol{v}}) - \Psi(\sum\limits_{k'}^{K} \lambda_{k'\boldsymbol{v}}) \\
&-& \sum\limits_{n}^{N} \sum\limits_{m}^{M} \mbrack{\rho_{mn} \log(\rho_{mn})}
+ \lambda \mparen{\sum\limits_{m}^{M}\rho_{mn} - 1 }
\end{eqnarray}

\begin{eqnarray}
\frac{\partial L}{\partial \rho_{mn}}
&=& \log(\eta) \\
&+& \log \delta_{g_{d_{mn}}^{\mathrm{d}}} - \frac{(x_{d_{mn}}^{\mathrm{d}} - x_n)^2 + (y_{d_{mn}}^{\mathrm{d}} - y_n)^2}{\sigma^2} \\
&+& \sum\limits_{k=1}^{K} \xi_{kn} \left[ \Psi(\gamma_{mn}) - \Psi(\sum\limits_{m'=1}^{M} \gamma_{m'n}) \right] \\
&+& \sum\limits_{k}^{K} \sum\limits_{v}^{V} \xi_{kn} w_n^v (\Psi(\lambda_{kv}) - \Psi(\sum\limits_{k'}^{K} \lambda_{k' \boldsymbol{v}}) \\
&-& \log(\rho_{mn}) - 1 + \lambda \stackrel{set}{=} 0 \\
\end{eqnarray}

Solving yields:
\[ \boxed{
\rho_{mn} \propto \eta \delta_{g_{d_{mn}}^{\mathrm{d}}} \frac{\exp \mparen{\sum\limits_{k=1}^{K} \xi_{kn}\mbrack{\Psi(\gamma_{mn}) - \Psi\mparen{\sum\limits_{m'=1}^{M} \gamma_{m'n}}} + \sum\limits_{k}^{K} \sum\limits_{v}^{V} \mbrack{\xi_{kn} w_n^v \mparen{\Psi(\lambda_{kv}) - \Psi\mparen{\sum\limits_{k'}^{K} \lambda_{k' \boldsymbol{v}}}}} }}
{\exp\mparen{\frac{(x_{d_{mn}}^{\mathrm{d}} - x_n)^2 + (y_{d_{mn}}^{\mathrm{d}} - y_n)^2}{\sigma^2}}}
} \]

\begin{eqnarray}
L_{\xi_{kn}}
&=& \sum\limits_{n=1}^{N} \sum\limits_{m=1}^{M} \sum\limits_{k=1}^{K} \rho_{mn} \xi_{kn} (\Psi(\gamma_{mk}) - \Psi(\sum\limits_{m'=1}^{M} \gamma_{m'k})) \\
&+& \sum\limits_{n}^{N} \sum\limits_{m}^{M} \sum\limits_{k}^{K} \sum\limits_{v}^{V} \rho_{mn} \xi_{kn} w_n^v (\Psi(\lambda_{k\boldsymbol{v}}) - \Psi(\sum\limits_{k'}^{K} \lambda_{k'\boldsymbol{v}})) \\
&-& \sum\limits_{n}^{N} \sum\limits_{k}^{K} \xi_{kn} \log(\xi_{kn}) + \lambda(\sum\limits_{k}^{K} \xi_{kn} - 1)\\
\end{eqnarray}

\begin{eqnarray}
\frac{\partial L}{\partial \xi_{kn}}
&=& \sum\limits_{m}^{M} \rho_{mn} \mparen{\Psi(\gamma_{mk}) - \Psi\mparen{\sum\limits_{m'=1}^{M} \gamma_{m'k}}} \\
&+& \sum\limits_{m}^{M} \sum\limits_{v}^{V} \rho_{mn} w_n^v \mparen{\Psi(\lambda_{k\boldsymbol{v}}) - \Psi\mparen{\sum\limits_{k'}^{K} \lambda_{k'\boldsymbol{v}}}} \\  
&-& \log(\xi_{kn}) - 1 + \lambda \stackrel{set}{=} 0
\end{eqnarray}

Similarly, solving yields:
\[ \boxed{
\xi_{kn} \propto \exp \mparen{\sum\limits_{m}^{M} \rho_{mn} \mparen{\Psi(\gamma_{mk}) - \Psi\mparen{\sum\limits_{m'=1}^{M} \gamma_{m'k}}} + \sum\limits_{m}^{M} \sum\limits_{v}^{V} \rho_{mn} w_n^v \mparen{\Psi(\lambda_{k\boldsymbol{v}}) - \Psi\mparen{\sum\limits_{k'}^{K} \lambda_{k'\boldsymbol{v}}}}}
} \]

\begin{eqnarray}
L_{\gamma_{mk}}
&=& \sum\limits_{m=1}^{M} \sum\limits_{k=1}^{K} (\alpha_{k}-1) \mparen{\Psi(\gamma_{mk}) - \Psi\mparen{\sum\limits_{k'=1}^{K} \gamma_{mk'}}}  \\
&+& \sum\limits_{n=1}^{N} \sum\limits_{m=1}^{M} \sum\limits_{k=1}^{K} \rho_{mn} \xi_{kn} \mparen {\Psi(\gamma_{mk}) - \Psi \mparen{\sum\limits_{m'=1}^{M} \gamma_{m'k}}} \\
&-& \sum\limits_{m}^{M} \mbrack{ \log \Gamma\mparen{ \sum\limits_{k}^{K} \gamma_{km}} - \sum\limits_{k}^{K} \log \Gamma(\gamma_{km}) + \sum\limits_{k}^{K}(\gamma_{km}-1)\mparen{\Psi(\gamma_{km}) - \Psi \mparen{\sum\limits_{k'}^{K} \gamma_{k'm}}}}\\
&=& \sum\limits_{m=1}^{M} \sum\limits_{k=1}^{K} \mparen{\Psi(\gamma_{mk}) - \Psi\mparen{\sum\limits_{k'=1}^{K} \gamma_{mk'}}}  
\mparen{ \alpha_{k} + \sum\limits_{n=1}^{N} \rho_{mn} \xi_{kn} - \gamma_{km} }\\
&-& \sum\limits_{m}^{M} \log \Gamma \mparen{\sum\limits_{k}^{K} \gamma_{km}} + \sum\limits_{m}^{M} \sum\limits_{k}^{K} \log \Gamma(\gamma_{km}) \\
\end{eqnarray}

\begin{eqnarray}
\frac{\partial L}{\partial \gamma_{mk}}
&=& \Psi^\prime(\gamma_{mk}) (\alpha_{k} + \sum\limits_{n=1}^{N} \rho_{mn} \xi_{kn} - \gamma_{mk})  \\
&-& \Psi^\prime\mparen{\sum\limits_{k'=1}^{K} \gamma_{mk'}} \sum\limits_{k'}^{K} (\alpha_{k'} + \sum\limits_{n=1}^{N} \rho_{mn} \xi_{k'n} - \gamma_{mk'}) \stackrel{set}{=} 0
\end{eqnarray}

Or:
\begin{eqnarray}
(\alpha_{mk} + \sum\limits_{n=1}^{N} \rho_{mn} \xi_{kn} - \gamma_{mk}) = \frac{\Psi^\prime\mparen{\sum\limits_{k'=1}^{K} \gamma_{mk'}}}{\Psi^\prime(\gamma_{mk})} \sum\limits_{k'}^{K} \mparen{\alpha_{k'} + \sum\limits_{n=1}^{N} \rho_{mn} \xi_{k'n} - \gamma_{mk'}}
\end{eqnarray}

Sum over k, yields:
\begin{eqnarray}
\sum_{k}^{K} \mparen{\alpha_{k} + \sum\limits_{n=1}^{N} \rho_{mn} \xi_{kn} - \gamma_{mk}} 
= \mparen{\sum_{k}^{K} \frac{\Psi^\prime\mparen{\sum\limits_{k'=1}^{K} \gamma_{mk'}}}{\Psi^\prime(\gamma_{mk})}} \sum\limits_{k'}^{K} \mparen{\alpha_{k'} + \sum\limits_{n=1}^{N} \rho_{mn} \xi_{k'n} - \gamma_{mk'}}
\end{eqnarray}

Or

\begin{eqnarray}
\sum_{k}^{K} \mparen{\alpha_{k} + \sum\limits_{n=1}^{N} \rho_{mn} \xi_{kn} - \gamma_{mk}} = 0
\end{eqnarray}

Replacing it in ... yields:

\[ \boxed{
\gamma_{mk} = \alpha_{k} + \sum\limits_{n=1}^{N} \rho_{mn} \xi_{kn}
} \]

\begin{eqnarray}
L_{\lambda_{kv}}
&=& \sum\limits_{k=1}^{K} \left\lbrack \sum\limits_{v=1}^{V} (\beta_{v}-1) (\Psi(\lambda_{kv}) - \Psi(\sum\limits_{v^'=1}^{V} \lambda_{kv^'})) \right\rbrack \\
&+& \sum\limits_{n}^{N} \sum\limits_{m}^{M} \sum\limits_{k}^{K} \sum\limits_{v}^{V} \rho_{mn} \xi_{kn} w_n^v (\Psi(\lambda_{k\boldsymbol{v}}) - \Psi(\sum\limits_{k'}^{K} \lambda_{k'\boldsymbol{v}})) \\
&-& \sum\limits_{k}^{K} \left\lbrack \log \Gamma \mparen{\sum\limits_{v}^{V} \lambda_{kv}} - \sum\limits_{v}^{V} \log(\Gamma(\lambda_{kv})) + \sum\limits_{v}^{V}(\lambda_{kv}-1)(\Psi(\lambda_{kv}) - \Psi(\sum\limits_{v'}^{V} \lambda_{kv'}) \right\rbrack \\
&=& \sum\limits_{k=1}^{K} \sum\limits_{v=1}^{V} \mparen{\Psi(\lambda_{kv}) - \Psi(\sum\limits_{v^'=1}^{V} \lambda_{kv^'})} \mparen{\beta_{v} + \sum\limits_{n}^{N} \sum\limits_{m}^{M} \rho_{mn} \xi_{kn} w_n^v - \lambda_{kv}} \\
&-& \sum\limits_{k}^{K} \left\lbrace \log \Gamma(\sum\limits_{v}^{V} \lambda_{kv}) - \sum\limits_{v}^{V} \log(\Gamma(\lambda_{kv})) \right\rbrace
\end{eqnarray}

\begin{eqnarray}
\frac{\partial L}{\partial \lambda_{kv}}
&=& \Psi^\prime(\lambda_{kv})(\beta_{v} + \sum\limits_{n}^{N} \sum\limits_{m}^{M} \rho_{mn} \xi_{kn} w_n^v - \lambda_{kv}) \\
&-&\Psi^\prime(\sum\limits_{v^'=1}^{V}\lambda_{kv'})\sum\limits_{v'}^{V} (\beta_{v'} + \sum\limits_{n}^{N} \sum\limits_{m}^{M} \rho_{mn} \xi_{kn} w_n^{v'} - \lambda_{kv'}) \stackrel{set}{=} 0
\end{eqnarray}

Similar to above, solving yields:

\[ \boxed{
\lambda_{kv} = \beta_{v} + \sum\limits_{n}^{N} \sum\limits_{m}^{M} \rho_{mn} \xi_{kn} w_n^v
} \]

\begin{eqnarray}
L_{\beta_{v}}
&=& \sum\limits_{k=1}^{K} \left\lbrack \log \Gamma(\sum\limits_{v=1}^{V} \beta_{v}) - \sum\limits_{v=1}^{V} \log \Gamma(\beta_{v}) + \sum\limits_{v=1}^{V} (\beta_{v}-1) (\Psi(\lambda_{kv}) - \Psi(\sum\limits_{v^'=1}^{V} \lambda_{kv^'})) \right\rbrack + \sum\limits_{k}^{K} \lambda_k \mparen{\sum\limits_{v}^{V} \beta_{v}-1} \\
\end{eqnarray}

\begin{eqnarray}
L_{\alpha}
&=& \sum\limits_{m=1}^{M} \left\lbrack \log(\Gamma(\sum\limits_{k=1}^{K} \alpha_{k})) - \sum\limits_{k=1}^{K} \log(\Gamma(\alpha_{k})) + \sum\limits_{k=1}^{K} (\alpha_{k}-1) (\Psi(\gamma_{mk}) - \Psi(\sum\limits_{k'=1}^{K} \gamma_{mk'})) \right\rbrack \\
\end{eqnarray}

\begin{eqnarray}
\frac{\partial L}{\partial \alpha_i} 
&=& M \mbrack{\Psi \mparen{\sum\limits_{k}^{K} \alpha_k} + \Psi\mparen{\alpha_i}} + \sum\limits_{m}^{M} \mbrack{ \Psi(\gamma_{mi}) - \Psi(\sum\limits_{k'=1}^{K} \gamma_{mk'})} 
\end{eqnarray}

Hessian: 
\begin{eqnarray}
\frac{\partial^2 L}{\partial \alpha_i \partial \alpha_j} 
&=& M \mbrack{\Psi^\prime \mparen{\sum\limits_{k}^{K} \alpha_k} - I\mbrack{i=j} \Psi^\prime(\alpha_i)}
\end{eqnarray}

\end{document}

